theories/Unification_issue.v
@@ -1,0 +1,39 @@
+From CTree Require Import 
+	CTrees Equ
+  .
+
+From Coinduction Require Import 
+	coinduction rel tactics.
+
+(* We work over a (coinductive) parameterized data-structure named `ctree E X`.
+	 We consider two different relations over this datatype, both 
+	 defined as greatest fixedpoint via the `coq-coinduction` library.
+
+		Here is a smallish example where unification goes wrong.
+	 *)
+Goal forall E X, (Reflexive (@equF E X X eq (gfp (fequ eq)))).
+	(* I currently have only one of the two relations in scope,
+		 that is the greatest fixedpoint of the `fequ` endofunction.
+		 Everything goes smoothly.
+	*)
+	intros.
+	typeclasses eauto. 
+	Restart.
+	(* Explicitely, the proof search finds the following proof *)
+	intros.
+  apply Reflexive_equF.
+	eauto.
+	apply (@Equivalence_Reflexive _ _ Equivalence_equ).
+	Restart.
+	intros.
+
+  From CTree Require Import Bisim.
+(* But now, when both relations are in scope, instances such as `Bisim.Reflexive_t` 
+	 lead to huge unification problems that eventually turn out impossible, allowing 
+	 the previous proof to finally be found, but only after an excruciating time.
+*)
+
+	Time typeclasses eauto.  (* ~30s on my machine *)
+
+Qed.
+
